theories/c_interface/notation.v
@@ -7,5 +7,5 @@ Coercion LitBool : bool >-> base_lit.
 Coercion LitLoc : loc >-> base_lit.
 
 (* No scope, does not conflict and scope is often not inferred properly. *)
-Notation "# l" := (LitV l%Z%V%stdpp) (at level 8, format "# l").
+Notation "# l" := (LitV l%Z%CV%stdpp) (at level 8, format "# l").
 Notation "& f" := (LitV (LitFunPtr f)) (at level 8, format "& f").
